iris/algebra/cmra.v
@@ -106,19 +106,6 @@ Global Hint Extern 0 (ValidN _) => refine (cmra_validN _); shelve : typeclass_in
 Coercion cmra_ofeO (A : cmra) : ofe := Ofe A (cmra_ofe_mixin A).
 Canonical Structure cmra_ofeO.
 
-(** As explained more thoroughly in iris#539, Coq can run into trouble when
-  [cmra] combinators (such as [optionUR]) are stacked and combined with
-  coercions like [cmra_ofeO]. To partially address this, we give Coq's
-  type-checker some directions for unfolding, with the Strategy command.
-
-  For these structures, we instruct Coq to eagerly _expand_ all projections,
-  except for the coercion to type (in this case, [cmra_car]), since that causes
-  problem with canonical structure inference. Additionally, we make Coq 
-  eagerly expand the coercions that go from one structure to another, like
-  [cmra_ofeO] in this case. *)
-Global Strategy expand [cmra_ofeO cmra_equiv cmra_dist cmra_pcore cmra_op
-                        cmra_valid cmra_validN cmra_ofe_mixin cmra_mixin].
-
 Definition cmra_mixin_of' A {Ac : cmra} (f : Ac → A) : CmraMixin Ac := cmra_mixin Ac.
 Notation cmra_mixin_of A :=
   ltac:(let H := eval hnf in (cmra_mixin_of' A id) in exact H) (only parsing).
@@ -208,24 +195,29 @@ Record UcmraMixin A `{!Dist A, !Equiv A, !PCore A, !Op A, !Valid A, !Unit A} := 
   mixin_ucmra_pcore_unit : pcore ε ≡@{option A} Some ε
 }.
 
-#[projections(primitive=no)] (* FIXME: making this primitive leads to strange
-TC resolution failures in view.v *)
+#[projections(primitive=yes)]
 Structure ucmra := Ucmra' {
-  ucmra_car :> Type;
-  ucmra_equiv : Equiv ucmra_car;
-  ucmra_dist : Dist ucmra_car;
-  ucmra_pcore : PCore ucmra_car;
-  ucmra_op : Op ucmra_car;
-  ucmra_valid : Valid ucmra_car;
-  ucmra_validN : ValidN ucmra_car;
-  ucmra_unit : Unit ucmra_car;
-  ucmra_ofe_mixin : OfeMixin ucmra_car;
-  ucmra_cmra_mixin : CmraMixin ucmra_car;
-  ucmra_mixin : UcmraMixin ucmra_car;
+  ucmra_cmraR :> cmra;
+  ucmra_unit : Unit (cmra_car ucmra_cmraR);
+  ucmra_mixin : UcmraMixin (cmra_car ucmra_cmraR);
 }.
-Global Arguments Ucmra' _ {_ _ _ _ _ _ _} _ _ _.
+(* This _reversible_ coercion allows us to infer [ucmra]s from [Type]s by using
+   Canonical instances. *)
+#[reversible] Coercion ucmra_car (u : ucmra) : Type := cmra_car (ucmra_cmraR u).
+
+(* Old projections for backwards compatibility *)
+Definition ucmra_equiv (u : ucmra) : Equiv (ucmra_car u) := cmra_equiv (ucmra_cmraR u).
+Definition ucmra_dist (u : ucmra) : Dist (ucmra_car u) := cmra_dist (ucmra_cmraR u).
+Definition ucmra_pcore (u : ucmra) : PCore (ucmra_car u) := cmra_pcore (ucmra_cmraR u).
+Definition ucmra_op (u : ucmra) : Op (ucmra_car u) := cmra_op (ucmra_cmraR u).
+Definition ucmra_valid (u : ucmra) : Valid (ucmra_car u) := cmra_valid (ucmra_cmraR u).
+Definition ucmra_validN (u : ucmra) : ValidN (ucmra_car u) := cmra_validN (ucmra_cmraR u).
+Definition ucmra_ofe_mixin (u : ucmra) : OfeMixin (ucmra_car u) := cmra_ofe_mixin (ucmra_cmraR u).
+Definition ucmra_cmra_mixin (u : ucmra) : CmraMixin (ucmra_car u) := cmra_mixin (ucmra_cmraR u).
+
+Global Arguments Ucmra' _ {_} _.
 Notation Ucmra A m :=
-  (Ucmra' A (ofe_mixin_of A%type) (cmra_mixin_of A%type) m) (only parsing).
+  (Ucmra' (A : cmra) m) (only parsing).
 Global Arguments ucmra_car : simpl never.
 Global Arguments ucmra_equiv : simpl never.
 Global Arguments ucmra_dist : simpl never.
@@ -239,20 +231,14 @@ Global Arguments ucmra_mixin : simpl never.
 Add Printing Constructor ucmra.
 (* FIXME(Coq #6294) : we need the new unification algorithm here. *)
 Global Hint Extern 0 (Unit _) => refine (ucmra_unit _); shelve : typeclass_instances.
-Coercion ucmra_ofeO (A : ucmra) : ofe := Ofe A (ucmra_ofe_mixin A).
-Canonical Structure ucmra_ofeO.
-Coercion ucmra_cmraR (A : ucmra) : cmra :=
-  Cmra' A (ucmra_ofe_mixin A) (ucmra_cmra_mixin A).
-Canonical Structure ucmra_cmraR.
 
-(** As for CMRAs above, we instruct Coq to eagerly _expand_ all projections,
-  except for the coercion to type (in this case, [ucmra_car]), since that causes
-  problem with canonical structure inference.  Additionally, we make Coq 
-  eagerly expand the coercions that go from one structure to another, like
-  [ucmra_cmraR] and [ucmra_ofeO] in this case. *)
-Global Strategy expand [ucmra_cmraR ucmra_ofeO ucmra_equiv ucmra_dist ucmra_pcore
-                        ucmra_op ucmra_valid ucmra_validN ucmra_unit
-                        ucmra_ofe_mixin ucmra_cmra_mixin].
+(* TODO: I do not think this is needed anywhere, since it is the compisition of two existing coercions?
+Coercion ucmra_ofeO (A : ucmra) : ofe := Ofe A (ucmra_ofe_mixin A).
+
+  TODO: I also don't know what these are supposed to do
+Canonical Structure ucmra_ofeO.
+Canonical Structure ucmra_cmraR.
+*)
 
 (** Lifting properties from the mixin *)
 Section ucmra_mixin.
